modélisation Isabelle/sync-mod/SyncModProof.thy
@@ -9,10 +9,168 @@ definition HOMachine_to_Algorithm :: "(Proc, pstate, SendVal) HOMachine \<Righta
 definition monovalent where
 "monovalent rho v n \<equiv> \<forall>p ss st. rho n p = Active ss \<longrightarrow> rho (Suc n) p = Active st \<longrightarrow> x st = v"
 
-lemma A1 : assumes "xi_nek HO xi"
-and run:"HORun (HOMachine_to_Algorithm SM_M) rho HO" (is "HORun ?A _ _")
+(*lemma A1 : assumes "rho r p = Active s"
+and run:"HORun (HOMachine_to_Algorithm (k_mod.SyncMod_HOMachine k)) rho HO" (is "HORun ?A _ _")
+and "x s = k-1"
+and "p \<in> HO (Suc r) q"
+and "rho r q \<noteq> Aslept"
+shows "\<forall>st. rho (Suc r) q = Active st \<longrightarrow> x st = 0"
+proof (rule+)
+    fix st
+    assume "rho (Suc r) q = Active st"
+    show "x st = 0"
+    proof -
+        *)
+
+lemma transition : assumes s_def:"rho r p = Active s"
+and ss_def:"rho (Suc r) p = Active ss"
+and run:"HORun (HOMachine_to_Algorithm (k_mod.SyncMod_HOMachine k)) rho HO" (is "HORun ?A _ _")
+shows "k_mod.SyncMod_nextState k p s (HOrcvdMsgs ?A p (HO (Suc r) p) (rho r)) ss" (is "k_mod.SyncMod_nextState  _ _ _ ?msgs _")
+proof -
+    have "CHOnextConfig ?A (rho r) (HO (Suc r)) (\<lambda>w. undefined) (rho (Suc r))" using run by (simp add:HORun_def CHORun_def)
+    then obtain sss where "rho (Suc r) p = Active sss \<and> CnextState ?A p s ?msgs undefined sss" 
+        using CHOnextConfig_def[of ?A "rho r" "HO (Suc r)" "\<lambda>w. undefined" "rho (Suc r)"] s_def by fastforce
+    hence "CnextState ?A p s ?msgs undefined ss" using ss_def by auto
+    thus ?thesis using HOMachine_to_Algorithm_def k_mod.SyncMod_HOMachine_def[of k] by (simp add:k_mod.simp_nextState)
+qed
+
+lemma stating : assumes "0 < n \<longrightarrow> rho (n-1) p = Aslept"
+and run:"HORun (HOMachine_to_Algorithm (k_mod.SyncMod_HOMachine k)) rho HO" (is "HORun ?A _ _")
+and "rho n p = Active s"
+shows "x s = k" and "\<forall>q. HOrcvdMsgs ?A q (HO (Suc n) q) (rho n) p = (if p \<in> HO (Suc n) q then Content Nope else Void)"
+proof -
+    have "CHOinitConfig ?A rho (\<lambda>w ww. undefined)"
+        using run HORun_def[of ?A rho HO] CHORun_def[of ?A rho HO "\<lambda>w ww. undefined"] by simp
+    hence "CinitState ?A p s undefined"
+        using CHOinitConfig_def[of ?A rho] \<open>rho n p = Active s\<close> \<open>0 < n \<longrightarrow> rho (n-1) p = Aslept\<close> by auto
+    hence "k_mod.SyncMod_initState k p s"
+        using HOMachine_to_Algorithm_def by (simp add:k_mod.SyncMod_HOMachine_def)
+    hence "x s = k" using k_mod.SyncMod_initState_def[of k p s] by auto
+    hence "\<forall>q. k_mod.SyncMod_sendMsg k p q s = Nope"
+        using k_mod.SyncMod_sendMsg_def[of k p _ s] by fastforce
+    hence "\<forall>q. sendMsg ?A p q s = Nope"
+        using HOMachine_to_Algorithm_def k_mod.SyncMod_HOMachine_def by (simp add: k_mod.SyncMod_HOMachine_def)
+    hence "\<forall>q. HOrcvdMsgs ?A q (HO (Suc n) q) (rho n) p = (if p \<in> HO (Suc n) q then Content Nope else Void)"
+        using HOrcvdMsgs_def[of ?A p "HO (Suc n) p" "rho n"] by (simp add: HOrcvdMsgs_def assms(3))
+    thus "x s = k" and "\<forall>q. HOrcvdMsgs ?A q (HO (Suc n) q) (rho n) p = (if p \<in> HO (Suc n) q then Content Nope else Void)"
+        using \<open>x s  = k\<close> by auto
+qed
+
+lemma A1 : assumes run:"HORun (HOMachine_to_Algorithm (k_mod.SyncMod_HOMachine k)) rho HO" (is "HORun ?A _ _")
+and "k > 2"
+shows "\<forall>r v p s ss. rho r p = Active s \<longrightarrow> rho (Suc r) p = Active ss \<longrightarrow> x ss = v \<longrightarrow> 0 \<le> v \<and> v < k"
+proof (rule allI)+
+    fix r v s ss p
+    show "rho r p = Active s \<longrightarrow> rho (Suc r) p = Active ss \<longrightarrow> x ss = v \<longrightarrow> 0 \<le> v \<and> v < k"
+    proof (induction r arbitrary:p v s ss)
+        case 0
+        show ?case
+        proof (rule impI)+
+            assume s_def:"rho 0 p = Active s"
+            assume ss_def:"rho (Suc 0) p = Active ss"
+            assume "x ss = v"
+            have no_content:"\<forall>v q. HOrcvdMsgs ?A p (HO 1 p) (rho 0) q \<noteq> Content (Val v)" (is "\<forall>v q. ?msgs q \<noteq> _")
+            proof (rule allI)+
+                fix v
+                fix q
+                show "?msgs q \<noteq> Content (Val v)"
+                proof (cases "rho 0 q")
+                    case "Aslept"
+                    hence "?msgs q = (if q \<in> HO 1 p then Bot else Void)" using HOrcvdMsgs_def[of ?A p "HO 1 p" "rho 0"] by auto
+                    thus "?msgs q \<noteq> Content (Val v)" by auto
+                next
+                    case (Active sq)
+                    hence "?msgs q = (if q \<in> HO 1 p then Content Nope else Void)"
+                        using stating[of 0 rho q k HO sq] run by auto
+                    thus "?msgs q \<noteq> Content (Val v)" by auto
+                qed
+            qed
+            hence "\<forall>v. \<not> k_mod.concordant ?msgs v" by (simp add: k_mod.concordant_def)
+            moreover have "k_mod.SyncMod_nextState k p s ?msgs ss"
+                using transition[of rho 0 p s ss k HO] s_def ss_def run  by auto
+            ultimately have v_possible:"if k_mod.ready_force k ?msgs s then x ss = k - 1 else if x ss = 0 then True else False" 
+            using k_mod.SyncMod_nextState_def[of k p s ?msgs ss] by fastforce
+            show "0 \<le> v \<and> v < k"
+            proof (cases "k_mod.ready_force k ?msgs s") 
+                case True
+                thus "0 \<le> v \<and> v < k" using v_possible \<open>x ss = v\<close> by (meson no_content k_mod.ready_force_def)
+            next
+                case False
+                hence "v = 0" using v_possible \<open>x ss = v\<close> by simp
+                thus "0 \<le> v \<and> v < k" using \<open>k > 2\<close> by auto
+            qed
+        qed
+    next
+        case (Suc r)
+        fix p
+        show "rho (Suc r) p = Active s \<longrightarrow> rho (Suc (Suc r)) p = Active ss \<longrightarrow> x ss = v \<longrightarrow> 0 \<le> v \<and> v < k"
+        proof (rule impI)+
+            assume "rho (Suc r) p = Active s"
+            assume "rho (Suc (Suc r)) p = Active ss"
+            assume "x ss = v"
+            have "\<forall>q vv. HOrcvdMsgs ?A p (HO (Suc (Suc r)) p) (rho (Suc r)) q = Content (Val vv) \<longrightarrow> 0 \<le> vv \<and> vv < k"
+                (is "\<forall>q vv. ?msgs q = _ \<longrightarrow> _")
+            proof (rule allI impI)+
+                fix q :: Proc
+                fix vv
+                assume "?msgs q = Content (Val vv)"
+                show "0 \<le> vv \<and> vv < k"
+                proof (cases "rho (Suc r) q")
+                    case Aslept
+                    hence "?msgs q = (if q \<in> HO (Suc (Suc r)) p then Bot else Void)"
+                        using HOrcvdMsgs_def[of ?A p "HO (Suc (Suc r)) p" "rho (Suc r)"] by auto
+                    thus "0 \<le> vv \<and> vv < k" using \<open>?msgs q = Content (Val vv)\<close> by auto
+                next
+                    case (Active sq)
+                    show "0 \<le> vv \<and> vv < k"
+                    proof (cases "rho r q")
+                        case Aslept
+                        hence "?msgs q = (if q \<in> HO (Suc r) p then Content Nope else Void)"
+                            using run stating[of "Suc r" rho q k HO sq] \<open>rho (Suc r) q = Active sq\<close>
+                            \<open>?msgs q = Content (Val vv)\<close> by auto
+                        thus "0 \<le> vv \<and> vv < k" using \<open>?msgs q = Content (Val vv)\<close> by auto
+                    next
+                        case (Active sqq)
+                        have "sendMsg ?A q p sq = Val vv"
+                            using HOrcvdMsgs_def[of ?A p "HO (Suc (Suc r)) p" "rho (Suc r)"] \<open>?msgs q = Content (Val vv)\<close>
+                            \<open>rho (Suc r) q = Active sq\<close> by auto
+                        hence "x sq = vv" using HOMachine_to_Algorithm_def k_mod.SyncMod_HOMachine_def by 
+                            (simp add: \<open>\<And>k. k_mod.SyncMod_HOMachine k \<equiv> \<lparr>CinitState = \<lambda>p st crd. k_mod.SyncMod_initState k p st,
+                            sendMsg = k_mod.SyncMod_sendMsg k,
+                            CnextState = \<lambda>p st msgs crd. k_mod.SyncMod_nextState k p st msgs,
+                            HOcommPerRd = k_mod.SyncMod_commPerRd, HOcommGlobal = k_mod.SyncMod_commGlobal,
+                            HOcommSchedule = k_mod.SyncMod_commSchedule\<rparr>\<close>
+                            k_mod.SyncMod_sendMsg_def)
+                        thus "0 \<le> vv \<and> vv < k"
+                            using Suc.IH[of q sqq sq] \<open>rho r q = Active sqq\<close> \<open>rho (Suc r) q = Active sq\<close> by auto
+                    qed
+                qed
+            qed
+
+            have trans:"k_mod.SyncMod_nextState k p s ?msgs ss"
+                using run \<open>rho (Suc r) p = Active s\<close> \<open>rho (Suc (Suc r)) p = Active ss\<close> transition by auto
+            thus "0 \<le> v \<and> v < k"
+            proof (cases "k_mod.ready_force k ?msgs s")
+                case True
+                hence "x ss = k - 1" using trans k_mod.SyncMod_nextState_def by auto
+                thus "0 \<le> v \<and> v < k" using \<open>x ss = v\<close> \<open>k > 2\<close> by auto
+            next
+                case non_force:False
+                show "0 \<le> v \<and> v < k"
+                proof (cases "x ss = 0")
+                    case True
+                    thus "0 \<le> v \<and> v < k" using \<open>x ss = v\<close> \<open>k > 2\<close> by auto
+                next
+                    case False
+                    hence "\<exists>q. ?msgs q = Content (Val ((x ss - 1) mod k))"
+                        using trans k_mod.concordant_def k_mod.SyncMod_nextState_def[of k p s ?msgs ss] non_force by auto
+
+
+lemma A2 : assumes "k_mod.xi_nek HO xi"
+and run:"HORun (HOMachine_to_Algorithm (k_mod.SyncMod_HOMachine k)) rho HO" (is "HORun ?A _ _")
 and "rho r xi = Active s"
 and "x s = k - 1"
+and "k > 2"
 shows "monovalent rho 0 r"
 proof -
     have "\<forall>p ss st. rho r p = Active ss \<longrightarrow> rho (Suc r) p = Active st \<longrightarrow> x st = 0"
@@ -23,15 +181,39 @@ proof -
         assume "rho r p = Active ss"
         assume "rho (Suc r) p = Active st"
         show "x st = 0"
-        proof -
-            have "CHOnextConfig ?A (rho r) (HO r) (\<lambda>q. undefined) (rho (Suc r))" 
-                using HORun_def CHORun_def run
-                by fastforce
-            hence "\<exists>st. CnextState ?A p ss (HOrcvdMsgs ?A p (HO (Suc r) p) (rho (Suc r))) undefined st"
-            using CHOnextConfig_def[of ?A "rho r" "HO r" _ "rho (Suc r)"] \<open>rho r p = Active ss\<close> by 
-                
-            hence "k_mod.concordant (HOrcvdMsgs ?A p (HO (Suc r) p) (rho (Suc r))) (k-1)"
-                using HOMachine_to_Algorithm_def k_mod.SyncMod_HOMachine_def k_mod.SyncMod_nextState_def CHOnextConfig_def
-                by 
+        proof (rule ccontr)
+            assume "x st \<noteq> 0"
+            let ?msgs = "HOrcvdMsgs ?A p (HO (Suc r) p) (rho r)"
+            have "k_mod.SyncMod_sendMsg k xi p s = Val (x s)"
+                using  k_mod.SyncMod_sendMsg_def[of k xi p s] \<open>x s = k - 1\<close> \<open>k > 2\<close> by simp
+            hence "sendMsg ?A xi p s = Val (x s)"
+                using HOMachine_to_Algorithm_def k_mod.SyncMod_HOMachine_def 
+                by (simp add: \<open>\<And>k. k_mod.SyncMod_HOMachine k \<equiv> \<lparr>CinitState = \<lambda>p st crd. k_mod.SyncMod_initState k p st,
+                sendMsg = k_mod.SyncMod_sendMsg k, CnextState = \<lambda>p st msgs crd. k_mod.SyncMod_nextState k p st msgs,
+                HOcommPerRd = k_mod.SyncMod_commPerRd, HOcommGlobal = k_mod.SyncMod_commGlobal,
+                HOcommSchedule = k_mod.SyncMod_commSchedule\<rparr>\<close>)
+            hence "?msgs xi = Content (Val (x s))"
+                using \<open>k_mod.xi_nek HO xi\<close> HOrcvdMsgs_def[of ?A p "HO (Suc r) p" "rho r"] \<open>rho r xi = Active s\<close>
+                k_mod.xi_nek_def[of HO xi] by auto
+            hence "\<not> (k_mod.ready_force k ?msgs ss)"
+                    using k_mod.ready_force_def[of k ?msgs ss] \<open>x s = k-1\<close> by auto
+
+            moreover have "CnextState ?A p ss ?msgs undefined st" 
+                using HORun_def CHORun_def run CHOnextConfig_def[of ?A "rho r" _ _ "rho (Suc r)"]
+                \<open>rho r p = Active ss\<close>
+                \<open>rho (Suc r) p = Active st\<close> by fastforce
+            hence "k_mod.SyncMod_nextState k p ss ?msgs st"
+                using HOMachine_to_Algorithm_def k_mod.SyncMod_HOMachine_def[of k]
+                by (simp add: k_mod.simp_nextState)
+            ultimately have "k_mod.concordant ?msgs ((x st - 1) mod k)"
+                using k_mod.SyncMod_nextState_def[of k p ss ?msgs st] \<open>x st \<noteq> 0\<close> 
+                by auto
+            hence "\<forall>vv. ?msgs xi = Content (Val vv) \<longrightarrow> vv = ((x st - 1) mod k)" 
+                using k_mod.concordant_def[of ?msgs "(x st - 1) mod k"] by auto
+            hence "k - 1 = (x st - 1) mod k"
+                using \<open>?msgs xi = Content (Val (x s))\<close> \<open>x s = k - 1\<close> by auto
+            hence "0 = x st" by 
+            hence "\<exists>tem. ?msgs tem = Content (Val (x st)) \<and> (\<forall>q vv. ?msgs q = Content (Val vv) \<longrightarrow> vv = (x st))"
+                using k_mod.concordant_def[of ?msgs] by auto
 
 end
